separated the parameters out of the module proper

Picinae_calling.v
@@ -1,4 +1,4 @@
- (* Picinae: Platform In Coq for INstruction Analysis of Executables       ZZM7DZ
+(* Picinae: Platform In Coq for INstruction Analysis of Executables       ZZM7DZ
                                                                           $MNDM7
    Copyright (c) 2021 Kevin W. Hamlen            ,,A??=P                 OMMNMZ+
    The University of Texas at Dallas         =:$ZZ$+ZZI                  7MMZMZ7
@@ -51,1027 +51,1088 @@ Open Scope bool.
 Open Scope list.
 Open Scope N.
 
-Module Type PICINAE_CALLING_DEFS (IL: PICINAE_IL) (TIL: PICINAE_STATICS IL).
-Import IL.
-Import TIL.
-Module PTheory := PicinaeTheory IL.
+Module Type PICINAE_CALLING_DEFS (IL: PICINAE_IL).
+  Import IL.
+  Parameter expeqb : forall (e1 e2 : exp), bool.
+  Parameter expeq : forall (e1 e2 : exp), Prop.
+  Axiom expeqb_expeq : forall e1 e2, expeqb e1 e2 = true <-> expeq e1 e2.
+  Axiom expeq_trans : forall e1 e2 e3 (HE1 : expeq e1 e2) (HE2 : expeq e2 e3),
+      expeq e1 e3.
+  Axiom expeq_refl : forall e, expeq e e.
+  Axiom expeq_symm : forall e1 e2 (HEq : expeq e1 e2), expeq e2 e1.
+  Axiom eval_expeq :
+    forall h st e1 e2 v (HEq : expeq e1 e2) (HE : eval_exp h st e1 v),
+      eval_exp h st e2 v.
+End PICINAE_CALLING_DEFS.
 
-Parameter expeqb : forall (e1 e2 : exp), bool.
-Parameter expeq : forall (e1 e2 : exp), Prop.
-Axiom expeqb_expeq : forall e1 e2, expeqb e1 e2 = true <-> expeq e1 e2.
-Axiom expeq_trans : forall e1 e2 e3 (HE1 : expeq e1 e2) (HE2 : expeq e2 e3),
-  expeq e1 e3.
-Axiom expeq_refl : forall e, expeq e e.
-Axiom expeq_symm : forall e1 e2 (HEq : expeq e1 e2), expeq e2 e1.
-Axiom eval_expeq :
-  forall h st e1 e2 v (HEq : expeq e1 e2) (HE : eval_exp h st e2 v),
-    eval_exp h st e1 v.
+Module PICINAE_CALLING (IL: PICINAE_IL) (DEFS : PICINAE_CALLING_DEFS IL).
+  Import IL.
+  Import DEFS.
+  Definition store_delta := alist var (option exp).
 
-Definition store_delta := alist var (option exp).
-
-Definition delta_lookup (l: store_delta) v : option exp :=
-  match assoc v l with
-  | Some (Some e) => Some e
-  | Some None => None
-  | None => Some (Var v)
-  end.
-
-Notation "f [[ x := y ]]" :=
-  (assoc_cons x y f) (at level 50, left associativity).
-
-Notation "f [[ v ]]" :=
-  (delta_lookup f v) (at level 50, left associativity).
-
-Definition delta_merge_var oe1 oe2 :=
-  match oe1,oe2 with
-  | Some e1,Some e2 => if expeqb e1 e2 then Some e1 else None
-  | None,_ | _,None => None
-  end.
-
-Fixpoint delta_merge' (d1 d2 : store_delta) vl :=
-  match vl with
-  | nil => nil
-  | v::vs => (delta_merge' d1 d2 vs) [[v:=delta_merge_var (d1[[v]]) (d2[[v]])]]
-  end.
-
-Definition delta_merge (d1 d2 : store_delta) :=
-  delta_merge' d1 d2 (map fst d1 ++ map fst d2).
-
-Definition delta_leb_var d1 d2 v :=
-  match d1[[v]],d2[[v]] with
-  | None,_ => true
-  | Some _,None => false
-  | Some e1,Some e2 => expeqb e1 e2
-  end.
-
-Definition delta_leb (d1 d2 : store_delta) :=
-  forallb (fun v => delta_leb_var d1 d2 v) (map fst d1 ++ map fst d2).
-
-Inductive absexit := AELoc (n : N) | AEExp (e : exp) | AEExn (n : N).
-
-Definition trace_state : Type := store_delta * absexit.
-
-Definition trace_state_res := option (list trace_state).
-
-Definition trace_result : Type := treeN store_delta * list trace_state.
-Definition trace_inter : Type := trace_result * list trace_state.
-
-Definition join_res {A} res1 res2 : option (list A) :=
-  match res1,res2 with
-  | Some p1,Some p2 => Some (p1 ++ p2)
-  | _,_ => None
-  end.
-
-Fixpoint subst_exp (d: store_delta) e : option exp :=
-  match e with
-  | Var v => d[[v]]
-  | Word _ _ => Some e
-  | Load e1 e2 en len =>
-      match subst_exp d e1,subst_exp d e2 with
-      | Some e1',Some e2' => Some (Load e1' e2' en len)
-      | _,_ => None
-      end
-  | Store e1 e2 e3 en len =>
-      match subst_exp d e1,subst_exp d e2,subst_exp d e3 with
-      | Some e1',Some e2',Some e3' => Some (Store e1' e2' e3' en len)
-      | _,_,_ => None
-      end
-  | BinOp op e1 e2 =>
-      match subst_exp d e1,subst_exp d e2 with
-      | Some e1',Some e2' => Some (BinOp op e1' e2')
-      | _,_ => None
-      end
-  | UnOp op e' =>
-      match subst_exp d e' with
-      | Some e'' => Some (UnOp op e'')
-      | _ => None
-      end
-  | Cast typ w e' =>
-      match subst_exp d e' with
-      | Some e'' => Some (Cast typ w e'')
-      | _ => None
-      end
-  | Let var val body =>
-      subst_exp (d[[var := subst_exp d val]]) body
-  | Unknown _ => None
-  | Ite e1 e2 e3 =>
-      match subst_exp d e1,subst_exp d e2,subst_exp d e3 with
-      | Some e1',Some e2',Some e3' => Some (Ite e1' e2' e3')
-      | _,_,_ => None
-      end
-  | Extract n1 n2 e' =>
-      match subst_exp d e' with
-      | Some e'' => Some (Extract n1 n2 e'')
-      | _ => None
-      end
-  | Concat e1 e2 =>
-      match subst_exp d e1,subst_exp d e2 with
-      | Some e1',Some e2' => Some (Concat e1' e2')
-      | _,_ => None
-      end
-  end.
-
-Definition exit_exp e :=
-  match e with
-  (* | Word n _ => AELoc n *)
-  | _ => AEExp e
-  end.
-
-Fixpoint trace_stmt
-         (q : stmt) (next : store_delta -> trace_state_res) (d : store_delta)
-  : trace_state_res :=
-  match q with
-  | Nop => next d
-  | Move v e => next (d[[v := subst_exp d e]])
-  | Jmp e =>
-      match subst_exp d e with
-      | Some e' => Some ((d,exit_exp e') :: nil)
-      | _ => None
-      end
-  | Exn n => Some ((d, AEExn n) :: nil)
-  | Seq q1 q2 => trace_stmt q1 (trace_stmt q2 next) d
-  | If _ q1 q2 => join_res (trace_stmt q1 next d) (trace_stmt q2 next d)
-  | Rep _ s => None
-  end.
-
-Definition trace_exit_res n d : trace_state_res := Some ((d,AELoc n)::nil).
-
-Definition odelta_leb od1 od2 :=
-  match od1,od2 with
-  | Some d1,Some d2 => delta_leb d1 d2
-  | None,Some _ => false
-  | _,None => true
-  end.
-
-Definition odelta_merge d1 od2 :=
-  match od2 with
-  | Some d2 => delta_merge d1 d2
-  | None => d1
-  end.
-
-Definition step_trace prog '((info,r) : trace_result) '((d,ae) : trace_state) :=
-  let skip := ((info,(d,ae)::r),nil) in
-  match ae with
-  (* | AEExp (Word n _) *)
-  | AELoc n =>
-      match prog n with
-      | None => skip
-      | Some (sz,q) =>
-          let odn := treeN_lookup info n in
-          if odelta_leb odn (Some d)
-          then ((info,r),nil)
-          else let d' := odelta_merge d odn in
-               match trace_stmt q (trace_exit_res (n + sz)) d' with
-               | None => skip
-               | Some t => ((treeN_update info n (Some d'),r),t)
-               end
-      end
-  | _ => skip
-  end.
-
-Definition delta_le (d1 d2 : store_delta) :=
-  forall v e (HV : d1[[v]] = Some e), exists e', d2[[v]] = Some e' /\ expeq e e'.
-
-Definition delta_eq d1 d2 := delta_le d1 d2 /\ delta_le d2 d1.
-
-Definition delta_models h d st st' :=
-  forall v ev val (HX : d[[v]] = Some ev) (HME : eval_exp h st ev val),
-    st' v = val.
-
-Definition trace_state_models_exit h '(d,ax) st st' x :=
-  delta_models h d st st' /\
-    match ax,x with
-    | AEExn n,Raise n'
-    | AELoc n,Exit n' => n = n'
-    | AEExp e',Exit n =>
-        forall n' w (HME : eval_exp h st e' (VaN n' w)), n = n'
-    | _,_ => False
+  Definition delta_lookup (l: store_delta) v : option exp :=
+    match assoc v l with
+    | Some (Some e) => Some e
+    | Some None => None
+    | None => Some (Var v)
     end.
 
-Definition trace_state_models_oexit h P ts st st' ox :=
-  match ox with
-  | Some x => trace_state_models_exit h ts st st' x
-  | None => P ts
-  end.
+  Notation "f [[ x := y ]]" :=
+    (assoc_cons x y f) (at level 50, left associativity).
 
-Definition trace_states_model h tsl st st' x :=
-  Exists (fun ts => trace_state_models_exit h ts st st' x) tsl.
+  Notation "f [[ v ]]" :=
+    (delta_lookup f v) (at level 50, left associativity).
 
-Definition trace_states_modelo h P tsl st st' ox :=
-  Exists (fun ts => trace_state_models_oexit h P ts st st' ox) tsl.
+  Definition delta_merge_var oe1 oe2 :=
+    match oe1,oe2 with
+    | Some e1,Some e2 => if expeqb e1 e2 then Some e1 else None
+    | None,_ | _,None => None
+    end.
 
-Definition info_models_loc h info n st st' :=
-  match treeN_lookup info n with
-  | Some d => delta_models h d st st'
-  | None => False
-  end.
+  Fixpoint delta_merge' (d1 d2 : store_delta) vl :=
+    match vl with
+    | nil => nil
+    | v::vs => (delta_merge' d1 d2 vs) [[v:=delta_merge_var (d1[[v]]) (d2[[v]])]]
+    end.
 
-Definition info_models_exit h info st st' x :=
-  match x with
-  | Raise _ => False
-  | Exit n => info_models_loc h info n st st'
-  end.
+  Definition delta_merge (d1 d2 : store_delta) :=
+    delta_merge' d1 d2 (map fst d1 ++ map fst d2).
 
-Definition exec_inter_prog h p a st time1 st' a' time2 st'' x :=
-  exec_prog h p a st time1 st' (Exit a') /\
-    exec_prog h p a' st' time2 st'' x.
+  Definition delta_leb_var d1 d2 v :=
+    match d1[[v]],d2[[v]] with
+    | None,_ => true
+    | Some _,None => false
+    | Some e1,Some e2 => expeqb e1 e2
+    end.
 
-Definition trace_result_models_exit h '(info,tsl) st st' x :=
-  info_models_exit h info st st' x \/ trace_states_model h tsl st st' x.
+  Definition delta_leb (d1 d2 : store_delta) :=
+    forallb (fun v => delta_leb_var d1 d2 v) (map fst d1 ++ map fst d2).
 
-Definition trace_result_consistent h '(info,tsl) p st :=
-  forall st' a st'' x sz q
-         (HInfo : info_models_loc h info a st st')
-         (HE : exec_stmt h st' q st'' x)
-         (HP : p st' a = Some (sz,q)),
-    trace_result_models_exit h (info,tsl) st st'' (exitof (a+sz) x).
+  Inductive absexit := AELoc (n : N) | AEExp (e : exp) | AEExn (n : N).
 
-Definition trace_inter_consistent h '((info,tsl1),tsl2) p st :=
-  trace_result_consistent h (info,tsl1 ++ tsl2) p st.
+  Definition trace_state : Type := store_delta * absexit.
 
-Theorem delta_le_match d1 d2 :
-  delta_le d1 d2 <->
-    forall v,
-      match d1[[v]] with
-      | Some e => exists e', d2[[v]] = Some e' /\ expeq e e'
-      | None => True
+  Definition trace_state_res := option (list trace_state).
+
+  Definition trace_result : Type := treeN store_delta * list trace_state.
+  Definition trace_inter : Type := trace_result * list trace_state.
+
+  Definition join_res {A} res1 res2 : option (list A) :=
+    match res1,res2 with
+    | Some p1,Some p2 => Some (p1 ++ p2)
+    | _,_ => None
+    end.
+
+  Fixpoint subst_exp (d: store_delta) e : option exp :=
+    match e with
+    | Var v => d[[v]]
+    | Word _ _ => Some e
+    | Load e1 e2 en len =>
+        match subst_exp d e1,subst_exp d e2 with
+        | Some e1',Some e2' => Some (Load e1' e2' en len)
+        | _,_ => None
+        end
+    | Store e1 e2 e3 en len =>
+        match subst_exp d e1,subst_exp d e2,subst_exp d e3 with
+        | Some e1',Some e2',Some e3' => Some (Store e1' e2' e3' en len)
+        | _,_,_ => None
+        end
+    | BinOp op e1 e2 =>
+        match subst_exp d e1,subst_exp d e2 with
+        | Some e1',Some e2' => Some (BinOp op e1' e2')
+        | _,_ => None
+        end
+    | UnOp op e' =>
+        match subst_exp d e' with
+        | Some e'' => Some (UnOp op e'')
+        | _ => None
+        end
+    | Cast typ w e' =>
+        match subst_exp d e' with
+        | Some e'' => Some (Cast typ w e'')
+        | _ => None
+        end
+    | Let var val body =>
+        subst_exp (d[[var := subst_exp d val]]) body
+    | Unknown _ => None
+    | Ite e1 e2 e3 =>
+        match subst_exp d e1,subst_exp d e2,subst_exp d e3 with
+        | Some e1',Some e2',Some e3' => Some (Ite e1' e2' e3')
+        | _,_,_ => None
+        end
+    | Extract n1 n2 e' =>
+        match subst_exp d e' with
+        | Some e'' => Some (Extract n1 n2 e'')
+        | _ => None
+        end
+    | Concat e1 e2 =>
+        match subst_exp d e1,subst_exp d e2 with
+        | Some e1',Some e2' => Some (Concat e1' e2')
+        | _,_ => None
+        end
+    end.
+
+  Definition exit_exp e :=
+    match e with
+    (* | Word n _ => AELoc n *)
+    | _ => AEExp e
+    end.
+
+  Fixpoint trace_stmt
+           (q : stmt) (next : store_delta -> trace_state_res) (d : store_delta)
+    : trace_state_res :=
+    match q with
+    | Nop => next d
+    | Move v e => next (d[[v := subst_exp d e]])
+    | Jmp e =>
+        match subst_exp d e with
+        | Some e' => Some ((d,exit_exp e') :: nil)
+        | _ => None
+        end
+    | Exn n => Some ((d, AEExn n) :: nil)
+    | Seq q1 q2 => trace_stmt q1 (trace_stmt q2 next) d
+    | If _ q1 q2 => join_res (trace_stmt q1 next d) (trace_stmt q2 next d)
+    | Rep _ s => None
+    end.
+
+  Definition trace_exit_res n d : trace_state_res := Some ((d,AELoc n)::nil).
+
+  Definition odelta_leb od1 od2 :=
+    match od1,od2 with
+    | Some d1,Some d2 => delta_leb d1 d2
+    | None,Some _ => false
+    | _,None => true
+    end.
+
+  Definition odelta_merge d1 od2 :=
+    match od2 with
+    | Some d2 => delta_merge d1 d2
+    | None => d1
+    end.
+
+  Definition step_trace prog '(info,r) '(d,ae) :=
+    let skip := ((info,(d,ae)::r),nil) in
+    match ae with
+    (* | AEExp (Word n _) *)
+    | AELoc n =>
+        match prog n with
+        | None => skip
+        | Some (sz,q) =>
+            let odn := treeN_lookup info n in
+            if odelta_leb odn (Some d)
+            then ((info,r),nil)
+            else let d' := odelta_merge d odn in
+                 match trace_stmt q (trace_exit_res (n + sz)) d' with
+                 | None => skip
+                 | Some t => ((treeN_update info n (Some d'),r),t)
+                 end
+        end
+    | _ => skip
+    end.
+
+  Definition delta_le (d1 d2 : store_delta) :=
+    forall v e (HV : d1[[v]] = Some e),
+    exists e', d2[[v]] = Some e' /\ expeq e e'.
+
+  Definition delta_eq d1 d2 := delta_le d1 d2 /\ delta_le d2 d1.
+
+  Definition delta_models h d st st' :=
+    forall v ev val (HX : d[[v]] = Some ev) (HME : eval_exp h st ev val),
+      st' v = val.
+
+  Definition trace_state_models_exit h '(d,ax) st st' x :=
+    delta_models h d st st' /\
+      match ax,x with
+      | AEExn n,Raise n'
+      | AELoc n,Exit n' => n = n'
+      | AEExp e',Exit n =>
+          forall n' w (HME : eval_exp h st e' (VaN n' w)), n = n'
+      | _,_ => False
       end.
-Proof.
-  unfold delta_le.
-  split; intros HX v; specialize (HX v);
-    [destruct (d1 [[v]]);try apply HX;tauto|].
-  intros e HV.
-  rewrite HV in HX.
-  assumption.
-Qed.
 
-Theorem delta_le_matchx d1 d2 :
-  delta_le d1 d2 <->
-    forall v,
-      match d1[[v]],d2[[v]] with
-      | Some e1,Some e2 => expeq e1 e2
-      | Some _,None => False
-      | None,_ => True
-      end.
-Proof.
-  unfold delta_le.
-  split; intros HX v; specialize (HX v).
-  {
-    destruct (d1 [[v]]);[|tauto].
-    destruct (HX _ eq_refl) as [? [HEq ?] ].
-    rewrite HEq.
-    assumption.
-  }
-  {
+  Definition trace_state_models_oexit h P ts st st' ox :=
+    match ox with
+    | Some x => trace_state_models_exit h ts st st' x
+    | None => P ts
+    end.
+
+  Definition trace_states_model h tsl st st' x :=
+    Exists (fun ts => trace_state_models_exit h ts st st' x) tsl.
+
+  Definition trace_states_modelo h P tsl st st' ox :=
+    Exists (fun ts => trace_state_models_oexit h P ts st st' ox) tsl.
+
+  Definition info_models_loc h info n st st' :=
+    match treeN_lookup info n with
+    | Some d => delta_models h d st st'
+    | None => False
+    end.
+
+  Definition info_models_exit h info st st' x :=
+    match x with
+    | Raise _ => False
+    | Exit n => info_models_loc h info n st st'
+    end.
+
+  Definition exec_inter_prog h p a st time1 st' a' time2 st'' x :=
+    exec_prog h p a st time1 st' (Exit a') /\
+      exec_prog h p a' st' time2 st'' x.
+
+  Definition trace_result_models_exit h '(info,tsl) st st' x :=
+    info_models_exit h info st st' x \/ trace_states_model h tsl st st' x.
+
+  Definition trace_result_consistent h '(info,tsl) p st :=
+    forall st' a st'' x sz q
+           (HInfo : info_models_loc h info a st st')
+           (HE : exec_stmt h st' q st'' x)
+           (HP : p st' a = Some (sz,q)),
+      trace_result_models_exit h (info,tsl) st st'' (exitof (a+sz) x).
+
+  Definition trace_inter_consistent h '((info,tsl1),tsl2) p st :=
+    trace_result_consistent h (info,tsl1 ++ tsl2) p st.
+
+  Theorem delta_le_match d1 d2 :
+    delta_le d1 d2 <->
+      forall v,
+        match d1[[v]] with
+        | Some e => exists e', d2[[v]] = Some e' /\ expeq e e'
+        | None => True
+        end.
+  Proof.
+    unfold delta_le.
+    split; intros HX v; specialize (HX v);
+      [destruct (d1 [[v]]);try apply HX;tauto|].
     intros e HV.
     rewrite HV in HX.
-    destruct (d2 [[v]]); [|tauto].
-    econstructor; split; [reflexivity|eassumption].
-  }
-Qed.
+    assumption.
+  Qed.
 
-Theorem delta_eq_alt d1 d2 :
-  delta_eq d1 d2 <->
-    forall v,
-      (d1[[v]] = None /\ d2[[v]] = None) \/
-        exists e1 e2,
-          d1[[v]] = Some e1 /\ d2[[v]] = Some e2 /\ expeq e1 e2.
-Proof.
-  unfold delta_eq.
-  repeat rewrite delta_le_match.
-  split; intro HX.
-  {
-    intro v.
-    destruct HX as [HX1 HX2].
-    specialize (HX1 v).
-    specialize (HX2 v).
-    destruct (d1 [[v]]).
+  Theorem delta_le_matchx d1 d2 :
+    delta_le d1 d2 <->
+      forall v,
+        match d1[[v]],d2[[v]] with
+        | Some e1,Some e2 => expeq e1 e2
+        | Some _,None => False
+        | None,_ => True
+        end.
+  Proof.
+    unfold delta_le.
+    split; intros HX v; specialize (HX v).
     {
-      destruct HX1 as [? [HX2X ?] ].
-      rewrite HX2X in HX2.
-      right.
-      rewrite HX2X.
-      do 2 econstructor.
-      repeat split; try reflexivity.
+      destruct (d1 [[v]]);[|tauto].
+      destruct (HX _ eq_refl) as [? [HEq ?] ].
+      rewrite HEq.
       assumption.
     }
     {
+      intros e HV.
+      rewrite HV in HX.
       destruct (d2 [[v]]); [|tauto].
-      destruct HX2 as [? [? ?] ].
+      econstructor; split; [reflexivity|eassumption].
+    }
+  Qed.
+
+  Theorem delta_eq_alt d1 d2 :
+    delta_eq d1 d2 <->
+      forall v,
+        (d1[[v]] = None /\ d2[[v]] = None) \/
+          exists e1 e2,
+            d1[[v]] = Some e1 /\ d2[[v]] = Some e2 /\ expeq e1 e2.
+  Proof.
+    unfold delta_eq.
+    repeat rewrite delta_le_match.
+    split; intro HX.
+    {
+      intro v.
+      destruct HX as [HX1 HX2].
+      specialize (HX1 v).
+      specialize (HX2 v).
+      destruct (d1 [[v]]).
+      {
+        destruct HX1 as [? [HX2X ?] ].
+        rewrite HX2X in HX2.
+        right.
+        rewrite HX2X.
+        do 2 econstructor.
+        repeat split; try reflexivity.
+        assumption.
+      }
+      {
+        destruct (d2 [[v]]); [|tauto].
+        destruct HX2 as [? [? ?] ].
+        discriminate.
+      }
+    }
+    {
+      split; intro v; specialize (HX v);
+        destruct HX as [ [HXD1 HXD2]|[? [? [HXD1 [HXD2 ?] ] ] ] ];
+        try rewrite HXD1; try rewrite HXD2; try tauto;
+        econstructor; split; try reflexivity; try assumption.
+      apply expeq_symm.
+      assumption.
+    }
+  Qed.
+
+  Theorem delta_le_leb d1 d2 (HL : delta_leb d1 d2 = true) : delta_le d1 d2.
+  Proof.
+    unfold delta_le,delta_leb,delta_leb_var,delta_lookup in *.
+    intros v e HV.
+    rewrite forallb_app in HL.
+    rewrite andb_true_iff in HL.
+    repeat rewrite forallb_forall in HL.
+    destruct HL as [HL1 HL2].
+    specialize (HL1 v).
+    specialize (HL2 v).
+    destruct (assoc v d1) as [ [?|]|] eqn:HA1;
+      [|discriminate|]; inversion HV; subst.
+    {
+      apply assoc_in in HA1.
+      apply (in_map fst) in HA1.
+      apply HL1 in HA1.
+      destruct (assoc v d2) as [ [?|]|] eqn:HA2; [|discriminate|];
+        econstructor; (split; [reflexivity|apply expeqb_expeq; eassumption]).
+    }
+    {
+      destruct (assoc v d2) as [o|] eqn:HA2.
+      {
+        apply assoc_in in HA2.
+        apply (in_map fst) in HA2.
+        apply HL2 in HA2.
+        destruct o; [|discriminate].
+        apply expeqb_expeq in HA2.
+        econstructor; (split; [reflexivity|eassumption]).
+      }
+      {
+        econstructor; (split; [reflexivity|]).
+        apply expeq_refl.
+      }
+    }
+  Qed.
+
+  Theorem delta_leb_le d1 d2 (HL : delta_le d1 d2) : delta_leb d1 d2 = true.
+  Proof.
+    unfold delta_le,delta_leb,delta_leb_var in *.
+    rewrite forallb_forall.
+    intros v HIn.
+    specialize (HL v).
+    destruct (d1 [[v]]); [|reflexivity].
+    destruct (HL _ eq_refl) as [? [HX ?] ].
+    rewrite HX.
+    apply expeqb_expeq.
+    assumption.
+  Qed.
+
+  Theorem delta_le_trans d1 d2 d3 (HL1 : delta_le d1 d2) (HL2 : delta_le d2 d3) :
+    delta_le d1 d3.
+  Proof.
+    unfold delta_le in *.
+    intros v e HV.
+    edestruct HL1 as [? [? ?] ]; [eassumption|].
+    edestruct HL2 as [? [? ?] ]; [eassumption|].
+    econstructor; split; [|eapply expeq_trans]; eassumption.
+  Qed.
+
+  Theorem delta_le_refl d : delta_le d d.
+  Proof.
+    intros v e HV.
+    exists e.
+    split; [eassumption|apply expeq_refl].
+  Qed.
+
+  Theorem delta_lookup_cons d v x k :
+    d [[v := x]] [[k]] = if k == v then x else d [[k]].
+  Proof.
+    unfold delta_lookup.
+    rewrite assoc_cons_lookup.
+    simpl.
+    destruct iseq; [|reflexivity].
+    destruct x; reflexivity.
+  Qed.
+
+  Theorem expeqb_symm e1 e2 : expeqb e1 e2 = expeqb e2 e1.
+  Proof.
+    destruct (expeqb e1 e2) eqn:HX1.
+    {
+      rewrite expeqb_expeq in HX1.
+      apply expeq_symm in HX1.
+      rewrite <- expeqb_expeq in HX1.
+      rewrite HX1.
+      reflexivity.
+    }
+    {
+      destruct (expeqb e2 e1) eqn:HX2; [|tauto].
+      rewrite expeqb_expeq in HX2.
+      apply expeq_symm in HX2.
+      rewrite <- expeqb_expeq in HX2.
+      rewrite HX1 in HX2.
       discriminate.
     }
-  }
-  {
-    split; intro v; specialize (HX v);
-      destruct HX as [ [HXD1 HXD2]|[? [? [HXD1 [HXD2 ?] ] ] ] ];
-      try rewrite HXD1; try rewrite HXD2; try tauto;
-      econstructor; split; try reflexivity; try assumption.
-    apply expeq_symm.
-    assumption.
-  }
-Qed.
+  Qed.
 
-Theorem delta_le_leb d1 d2 (HL : delta_leb d1 d2 = true) : delta_le d1 d2.
-Proof.
-  unfold delta_le,delta_leb,delta_leb_var,delta_lookup in *.
-  intros v e HV.
-  rewrite forallb_app in HL.
-  rewrite andb_true_iff in HL.
-  repeat rewrite forallb_forall in HL.
-  destruct HL as [HL1 HL2].
-  specialize (HL1 v).
-  specialize (HL2 v).
-  destruct (assoc v d1) as [ [?|]|] eqn:HA1;
-    [|discriminate|]; inversion HV; subst.
-  {
-    apply assoc_in in HA1.
-    apply (in_map fst) in HA1.
-    apply HL1 in HA1.
-    destruct (assoc v d2) as [ [?|]|] eqn:HA2; [|discriminate|];
-      econstructor; (split; [reflexivity|apply expeqb_expeq; eassumption]).
-  }
-  {
-    destruct (assoc v d2) as [o|] eqn:HA2.
-    {
-      apply assoc_in in HA2.
-      apply (in_map fst) in HA2.
-      apply HL2 in HA2.
-      destruct o; [|discriminate].
-      apply expeqb_expeq in HA2.
-      econstructor; (split; [reflexivity|eassumption]).
-    }
-    {
-      econstructor; (split; [reflexivity|]).
-      apply expeq_refl.
-    }
-  }
-Qed.
-
-Theorem delta_leb_le d1 d2 (HL : delta_le d1 d2) : delta_leb d1 d2 = true.
-Proof.
-  unfold delta_le,delta_leb,delta_leb_var in *.
-  rewrite forallb_forall.
-  intros v HIn.
-  specialize (HL v).
-  destruct (d1 [[v]]); [|reflexivity].
-  destruct (HL _ eq_refl) as [? [HX ?] ].
-  rewrite HX.
-  apply expeqb_expeq.
-  assumption.
-Qed.
-
-Theorem delta_le_trans d1 d2 d3 (HL1 : delta_le d1 d2) (HL2 : delta_le d2 d3) :
-  delta_le d1 d3.
-Proof.
-  unfold delta_le in *.
-  intros v e HV.
-  edestruct HL1 as [? [? ?] ]; [eassumption|].
-  edestruct HL2 as [? [? ?] ]; [eassumption|].
-  econstructor; split; [|eapply expeq_trans]; eassumption.
-Qed.
-
-Theorem delta_le_refl d : delta_le d d.
-Proof.
-  intros v e HV.
-  exists e.
-  split; [eassumption|apply expeq_refl].
-Qed.
-
-Theorem delta_lookup_cons d v x k :
-  d [[v := x]] [[k]] = if k == v then x else d [[k]].
-Proof.
-  unfold delta_lookup.
-  rewrite assoc_cons_lookup.
-  simpl.
-  destruct iseq; [|reflexivity].
-  destruct x; reflexivity.
-Qed.
-
-Theorem expeqb_symm e1 e2 : expeqb e1 e2 = expeqb e2 e1.
-Proof.
-  destruct (expeqb e1 e2) eqn:HX1.
-  {
-    rewrite expeqb_expeq in HX1.
-    apply expeq_symm in HX1.
-    rewrite <- expeqb_expeq in HX1.
-    rewrite HX1.
-    reflexivity.
-  }
-  {
-    destruct (expeqb e2 e1) eqn:HX2; [|tauto].
-    rewrite expeqb_expeq in HX2.
-    apply expeq_symm in HX2.
-    rewrite <- expeqb_expeq in HX2.
-    rewrite HX1 in HX2.
-    discriminate.
-  }
-Qed.
-
-Theorem delta_merge'_in d1 d2 vl v (HIn : In v vl) :
+  Theorem delta_merge'_in d1 d2 vl v (HIn : In v vl) :
     match (delta_merge' d1 d2 vl) [[v]],d1 [[v]],d2 [[v]] with
     | Some e,Some e1,Some e2 => expeq e e1 /\ expeq e1 e2
     | None,Some e1,Some e2 => ~ expeq e1 e2
     | Some _,None,_ | Some _,_,None => False
     | None,None,_ | None,_,None => True
     end.
-Proof.
-  induction vl; simpl in HIn; [tauto|].
-  simpl.
-  rewrite delta_lookup_cons.
-  destruct iseq; subst; [|apply IHvl;destruct HIn;subst;tauto].
-  unfold delta_merge_var.
-  destruct (d1 [[a]]),(d2 [[a]]); try tauto.
-  destruct expeqb eqn:HX; [|rewrite <- expeqb_expeq,HX;discriminate].
-  split; [apply expeq_refl|].
-  rewrite expeqb_expeq in HX.
-  assumption.
-Qed.
-
-Theorem delta_merge'_notin' d1 d2 vl v (HNIn : ~In v vl) :
-  assoc v (delta_merge' d1 d2 vl) = None.
-Proof.
-  induction vl; [reflexivity|].
-  simpl in *.
-  rewrite assoc_remove_lookup.
-  destruct iseq; subst; tauto.
-Qed.
-
-Theorem delta_merge'_notin d1 d2 vl v (HNIn : ~In v vl) :
-  (delta_merge' d1 d2 vl) [[v]] = Some (Var v).
-Proof.
-  unfold delta_lookup.
-  rewrite delta_merge'_notin' by assumption.
-  reflexivity.
-Qed.
-
-Theorem delta_merge'_symm' d1 d2 vl :
-  delta_le (delta_merge' d1 d2 vl) (delta_merge' d2 d1 vl).
-Proof.
-  unfold delta_le.
-  intros v e HV.
-  destruct (in_dec iseq v vl) as [HX1|HX1]; assert (HX2 := HX1);
-    [apply (delta_merge'_in d1 d2) in HX1
-    |apply (delta_merge'_notin d1 d2) in HX1];
-    rewrite HV in *; clear HV.
-  {
-    apply (delta_merge'_in d2 d1) in HX2.
-    destruct (d1 [[v]]) as [e1|],(d2 [[v]]) as [e2|]; try tauto.
-    destruct (delta_merge' _ _ _ [[v]]);
-      [|destruct HX2; apply expeq_symm; tauto].
-    econstructor.
-    split; [reflexivity|].
-    eapply expeq_trans; [apply HX1|].
-    apply expeq_symm.
-    eapply expeq_trans; apply HX2.
-  }
-  {
-    inversion HX1; subst.
-    rewrite delta_merge'_notin by assumption.
-    econstructor.
-    split; [reflexivity|apply expeq_refl].
-  }
-Qed.
-
-Theorem delta_merge'_symm d1 d2 vl :
-  delta_eq (delta_merge' d1 d2 vl) (delta_merge' d2 d1 vl).
-Proof.
-  split; apply delta_merge'_symm'.
-Qed.
-
-Theorem delta_merge'_le_l d1 d2 vl
-        (HIn : forall v, In v (map fst d1) -> In v vl) :
-  delta_le (delta_merge' d1 d2 vl) d1.
-Proof.
-  unfold delta_le.
-  intros v e HV.
-  destruct (in_dec iseq v vl) as [HX|HX].
-  {
-    apply (delta_merge'_in d1 d2) in HX.
-    rewrite HV in HX.
-    destruct (d1 [[v]]),(d2 [[v]]); try tauto.
-    destruct HX.
-    econstructor.
-    split; [reflexivity|].
+  Proof.
+    induction vl; simpl in HIn; [tauto|].
+    simpl.
+    rewrite delta_lookup_cons.
+    destruct iseq; subst; [|apply IHvl;destruct HIn;subst;tauto].
+    unfold delta_merge_var.
+    destruct (d1 [[a]]),(d2 [[a]]); try tauto.
+    destruct expeqb eqn:HX; [|rewrite <- expeqb_expeq,HX;discriminate].
+    split; [apply expeq_refl|].
+    rewrite expeqb_expeq in HX.
     assumption.
-  }
-  {
-    rewrite delta_merge'_notin in HV by assumption.
-    inversion HV; subst.
+  Qed.
+
+  Theorem delta_merge'_notin' d1 d2 vl v (HNIn : ~In v vl) :
+    assoc v (delta_merge' d1 d2 vl) = None.
+  Proof.
+    induction vl; [reflexivity|].
+    simpl in *.
+    rewrite assoc_remove_lookup.
+    destruct iseq; subst; tauto.
+  Qed.
+
+  Theorem delta_merge'_notin d1 d2 vl v (HNIn : ~In v vl) :
+    (delta_merge' d1 d2 vl) [[v]] = Some (Var v).
+  Proof.
     unfold delta_lookup.
-    destruct assoc eqn:HA;
-      [|econstructor; split; [reflexivity|apply expeq_refl] ].
-    apply assoc_in in HA.
-    eapply (in_map fst) in HA.
-    specialize (HIn v).
-    tauto.
-  }
-Qed.
+    rewrite delta_merge'_notin' by assumption.
+    reflexivity.
+  Qed.
 
-Theorem delta_merge_le_l d1 d2 : delta_le (delta_merge d1 d2) d1.
-Proof.
-  eapply delta_merge'_le_l.
-  intros.
-  apply in_or_app.
-  tauto.
-Qed.
-
-Theorem delta_merge_le_r d1 d2 : delta_le (delta_merge d1 d2) d2.
-Proof.
-  unfold delta_merge.
-  eapply delta_le_trans; [apply delta_merge'_symm|].
-  eapply delta_merge'_le_l.
-  intros.
-  apply in_or_app.
-  tauto.
-Qed.
-
-Theorem delta_merge_glb d1 d2 dx (HL1 : delta_le dx d1) (HL2 : delta_le dx d2) :
-  delta_le dx (delta_merge d1 d2).
-Proof.
-  unfold delta_le in *.
-  intros v e HV.
-  specialize (HL1 v e HV).
-  specialize (HL2 v e HV).
-  clear dx HV.
-  unfold delta_merge.
-  destruct HL1 as [? [HD1 HL1X] ], HL2 as [? [HD2 HL2X] ].
-  destruct (in_dec iseq v (map fst d1 ++ map fst d2)) as [HX|HX].
-  {
-    apply (delta_merge'_in d1 d2) in HX.
-    rewrite HD1,HD2 in HX.
-    destruct (delta_merge' _ _ _ [[v]]); destruct HX.
+  Theorem delta_merge'_symm' d1 d2 vl :
+    delta_le (delta_merge' d1 d2 vl) (delta_merge' d2 d1 vl).
+  Proof.
+    unfold delta_le.
+    intros v e HV.
+    destruct (in_dec iseq v vl) as [HX1|HX1]; assert (HX2 := HX1);
+      [apply (delta_merge'_in d1 d2) in HX1
+      |apply (delta_merge'_notin d1 d2) in HX1];
+      rewrite HV in *; clear HV.
     {
+      apply (delta_merge'_in d2 d1) in HX2.
+      destruct (d1 [[v]]) as [e1|],(d2 [[v]]) as [e2|]; try tauto.
+      destruct (delta_merge' _ _ _ [[v]]);
+        [|destruct HX2; apply expeq_symm; tauto].
       econstructor.
       split; [reflexivity|].
-      eapply expeq_trans; [apply HL1X|].
+      eapply expeq_trans; [apply HX1|].
       apply expeq_symm.
+      eapply expeq_trans; apply HX2.
+    }
+    {
+      inversion HX1; subst.
+      rewrite delta_merge'_notin by assumption.
+      econstructor.
+      split; [reflexivity|apply expeq_refl].
+    }
+  Qed.
+
+  Theorem delta_merge'_symm d1 d2 vl :
+    delta_eq (delta_merge' d1 d2 vl) (delta_merge' d2 d1 vl).
+  Proof.
+    split; apply delta_merge'_symm'.
+  Qed.
+
+  Theorem delta_merge'_le_l d1 d2 vl
+          (HIn : forall v, In v (map fst d1) -> In v vl) :
+    delta_le (delta_merge' d1 d2 vl) d1.
+  Proof.
+    unfold delta_le.
+    intros v e HV.
+    destruct (in_dec iseq v vl) as [HX|HX].
+    {
+      apply (delta_merge'_in d1 d2) in HX.
+      rewrite HV in HX.
+      destruct (d1 [[v]]),(d2 [[v]]); try tauto.
+      destruct HX.
+      econstructor.
+      split; [reflexivity|].
       assumption.
     }
     {
+      rewrite delta_merge'_notin in HV by assumption.
+      inversion HV; subst.
+      unfold delta_lookup.
+      destruct assoc eqn:HA;
+        [|econstructor; split; [reflexivity|apply expeq_refl] ].
+      apply assoc_in in HA.
+      eapply (in_map fst) in HA.
+      specialize (HIn v).
+      tauto.
+    }
+  Qed.
+
+  Theorem delta_merge_le_l d1 d2 : delta_le (delta_merge d1 d2) d1.
+  Proof.
+    eapply delta_merge'_le_l.
+    intros.
+    apply in_or_app.
+    tauto.
+  Qed.
+
+  Theorem delta_merge_le_r d1 d2 : delta_le (delta_merge d1 d2) d2.
+  Proof.
+    unfold delta_merge.
+    eapply delta_le_trans; [apply delta_merge'_symm|].
+    eapply delta_merge'_le_l.
+    intros.
+    apply in_or_app.
+    tauto.
+  Qed.
+
+  Theorem delta_merge_glb d1 d2 dx (HL1 : delta_le dx d1) (HL2 : delta_le dx d2) :
+    delta_le dx (delta_merge d1 d2).
+  Proof.
+    unfold delta_le in *.
+    intros v e HV.
+    specialize (HL1 v e HV).
+    specialize (HL2 v e HV).
+    clear dx HV.
+    unfold delta_merge.
+    destruct HL1 as [? [HD1 HL1X] ], HL2 as [? [HD2 HL2X] ].
+    destruct (in_dec iseq v (map fst d1 ++ map fst d2)) as [HX|HX].
+    {
+      apply (delta_merge'_in d1 d2) in HX.
+      rewrite HD1,HD2 in HX.
+      destruct (delta_merge' _ _ _ [[v]]); destruct HX.
+      {
+        econstructor.
+        split; [reflexivity|].
+        eapply expeq_trans; [apply HL1X|].
+        apply expeq_symm.
+        assumption.
+      }
+      {
+        eapply expeq_trans; [|eassumption].
+        apply expeq_symm.
+        assumption.
+      }
+    }
+    {
+      rewrite delta_merge'_notin by assumption.
+      econstructor.
+      split; [reflexivity|].
+      unfold delta_lookup in HD1.
+      destruct assoc eqn:HIn; [|inversion HD1; subst; assumption].
+      destruct HX.
+      apply in_or_app.
+      apply assoc_in in HIn.
+      apply (in_map fst) in HIn.
+      left.
+      assumption.
+    }
+  Qed.
+
+  Theorem delta_models_match h d st st' :
+    delta_models h d st st' <->
+      forall v,
+        match d[[v]] with
+        | Some ev => forall val, eval_exp h st ev val -> st' v = val
+        | None => True
+        end.
+  Proof.
+    unfold delta_models.
+    split; intro HM; intro v; specialize (HM v).
+    {
+      destruct (d [[v]]); [|tauto].
+      intro; apply HM.
+      reflexivity.
+    }
+    {
+      intros.
+      rewrite HX in HM.
+      apply HM,HME.
+    }
+  Qed.
+
+  Theorem delta_models_le h d1 d2 st st'
+          (HL : delta_le d1 d2) (HM : delta_models h d2 st st') :
+    delta_models h d1 st st'.
+  Proof.
+    rewrite delta_models_match,delta_le_matchx in *.
+    intro.
+    specialize (HM v).
+    specialize (HL v).
+    destruct (d1 [[v]]); [|apply I].
+    destruct (d2 [[v]]); [|tauto].
+    intros.
+    apply HM.
+    eapply eval_expeq; eassumption.
+  Qed.
+
+  Theorem delta_merge_witness' d1 d2 v :
+    match delta_merge d1 d2 [[v]],d1 [[v]],d2 [[v]] with
+    | Some e,Some e1,Some e2 => expeq e e1 /\ expeq e1 e2
+    | None,Some e1,Some e2 => ~ expeq e1 e2
+    | Some _,None,_ | Some _,_,None => False
+    | None,None,_ | None,_,None => True
+    end.
+  Proof.
+    assert (HD1 := delta_merge_le_l d1 d2).
+    assert (HD2 := delta_merge_le_r d1 d2).
+    rewrite delta_le_matchx in *.
+    specialize (HD1 v).
+    specialize (HD2 v).
+    destruct (d1 [[v]]) as [e|] eqn:HD1X, (d2 [[v]]) eqn:HD2X,
+            (delta_merge d1 d2 [[v]]) eqn:HDMX; try tauto.
+    {
+      split; [assumption|].
       eapply expeq_trans; [|eassumption].
       apply expeq_symm.
       assumption.
     }
-  }
-  {
-    rewrite delta_merge'_notin by assumption.
-    econstructor.
-    split; [reflexivity|].
-    unfold delta_lookup in HD1.
-    destruct assoc eqn:HIn; [|inversion HD1; subst; assumption].
-    destruct HX.
-    apply in_or_app.
-    apply assoc_in in HIn.
-    apply (in_map fst) in HIn.
-    left.
-    assumption.
-  }
-Qed.
-
-Theorem delta_models_match h d st st' :
-  delta_models h d st st' <->
-    forall v,
-      match d[[v]] with
-      | Some ev => forall val, eval_exp h st ev val -> st' v = val
-      | None => True
-      end.
-Proof.
-  unfold delta_models.
-  split; intro HM; intro v; specialize (HM v).
-  {
-    destruct (d [[v]]); [|tauto].
-    intro; apply HM.
-    reflexivity.
-  }
-  {
-    intros.
-    rewrite HX in HM.
-    apply HM,HME.
-  }
-Qed.
-
-Theorem delta_models_le h d1 d2 st st'
-        (HL : delta_le d1 d2) (HM : delta_models h d2 st st') :
-  delta_models h d1 st st'.
-Proof.
-  rewrite delta_models_match,delta_le_matchx in *.
-  intro.
-  specialize (HM v).
-  specialize (HL v).
-  destruct (d1 [[v]]); [|apply I].
-  destruct (d2 [[v]]); [|tauto].
-  intros.
-  apply HM.
-  eapply eval_expeq; [|eassumption].
-  apply expeq_symm.
-  assumption.
-Qed.
-
-Theorem delta_merge_witness' d1 d2 v :
-  match delta_merge d1 d2 [[v]],d1 [[v]],d2 [[v]] with
-  | Some e,Some e1,Some e2 => expeq e e1 /\ expeq e1 e2
-  | None,Some e1,Some e2 => ~ expeq e1 e2
-  | Some _,None,_ | Some _,_,None => False
-  | None,None,_ | None,_,None => True
-  end.
-Proof.
-  assert (HD1 := delta_merge_le_l d1 d2).
-  assert (HD2 := delta_merge_le_r d1 d2).
-  rewrite delta_le_matchx in *.
-  specialize (HD1 v).
-  specialize (HD2 v).
-  destruct (d1 [[v]]) as [e|] eqn:HD1X, (d2 [[v]]) eqn:HD2X,
-        (delta_merge d1 d2 [[v]]) eqn:HDMX; try tauto.
-  {
-    split; [assumption|].
-    eapply expeq_trans; [|eassumption].
-    apply expeq_symm.
-    assumption.
-  }
-  {
-    intro HEq.
-    assert (HM : delta_le (delta_merge d1 d2 [[v := Some e]])
-                          (delta_merge d1 d2)).
     {
-      apply delta_merge_glb; apply delta_le_matchx;
-        intro v'; rewrite delta_lookup_cons;
-        (destruct iseq; subst; [|apply delta_le_matchx]);
-        [rewrite HD1X;apply expeq_refl|apply delta_merge_le_l
-        |rewrite HD2X;assumption|apply delta_merge_le_r].
+      intro HEq.
+      assert (HM : delta_le (delta_merge d1 d2 [[v := Some e]])
+                            (delta_merge d1 d2)).
+      {
+        apply delta_merge_glb; apply delta_le_matchx;
+          intro v'; rewrite delta_lookup_cons;
+          (destruct iseq; subst; [|apply delta_le_matchx]);
+          [rewrite HD1X;apply expeq_refl|apply delta_merge_le_l
+          |rewrite HD2X;assumption|apply delta_merge_le_r].
+      }
+      rewrite delta_le_matchx in HM.
+      specialize (HM v).
+      rewrite delta_lookup_cons,HDMX in HM.
+      destruct iseq; tauto.
     }
-    rewrite delta_le_matchx in HM.
-    specialize (HM v).
-    rewrite delta_lookup_cons,HDMX in HM.
-    destruct iseq; tauto.
-  }
-Qed.
+  Qed.
 
-Theorem delta_merge_witness d1 d2 v e1 e2
-        (HD1 : d1 [[v]] = Some e1)
-        (HD2 : d2 [[v]] = Some e2)
-        (HEq : expeq e1 e2) :
-  exists em, delta_merge d1 d2 [[v]] = Some em /\ expeq em e1 /\ expeq e1 e2.
-Proof.
-  assert (HW := delta_merge_witness' d1 d2 v).
-  rewrite HD1,HD2 in HW.
-  destruct (delta_merge d1 d2 [[v]]); [|tauto].
-  econstructor; split; [reflexivity|].
-  tauto.
-Qed.
+  Theorem delta_merge_witness d1 d2 v e1 e2
+          (HD1 : d1 [[v]] = Some e1)
+          (HD2 : d2 [[v]] = Some e2)
+          (HEq : expeq e1 e2) :
+    exists em, delta_merge d1 d2 [[v]] = Some em /\ expeq em e1 /\ expeq e1 e2.
+  Proof.
+    assert (HW := delta_merge_witness' d1 d2 v).
+    rewrite HD1,HD2 in HW.
+    destruct (delta_merge d1 d2 [[v]]); [|tauto].
+    econstructor; split; [reflexivity|].
+    tauto.
+  Qed.
 
-Theorem subst_exp_model' h d s s' e val
-        (HST : delta_models h d s s')
-        (HE1 : eval_exp h s' e val) :
-  match subst_exp d e with
-  | Some e' => forall val' (HE2 : eval_exp h s e' val'), val = val'
-  | None => True
-  end.
-Proof.
-  rewrite delta_models_match in *.
-  revert d s HST.
-  induction HE1; simpl; intros.
-  1: {
-    apply HST.
-  }
-  7: {
-    apply IHHE1_2.
-    intro v'.
-    rewrite delta_lookup_cons in *.
-    destruct iseq; subst; [|rewrite update_frame by assumption; apply HST].
-    rewrite update_updated.
-    apply IHHE1_1.
-    assumption.
-  }
-  all:
-    repeat match goal with
-           | [IH : forall d _ _, match subst_exp d ?e with _ => _ end |- _] =>
-               specialize (IH _ _ HST)
-           end.
-  8: destruct n1.
-  all:
-    repeat match goal with
-           | [|- context [match subst_exp _ _ with _ => _ end] ] =>
-               destruct subst_exp
-           end; try solve [apply I].
-  all: intros; inversion HE2; subst.
-  all:
-    repeat match goal with
-           | [IH : forall _, (eval_exp _ _ ?e _) -> _ = _,
-                E : eval_exp _ _ ?e _ |- _] =>
-               specialize (IH _ E); inversion IH; subst
-           end; reflexivity.
-Qed.
-
-Theorem subst_exp_model h d s s' e val e' val'
-        (HST : delta_models h d s s')
-        (HS : subst_exp d e = Some e')
-        (HE1 : eval_exp h s' e val)
-        (HE2 : eval_exp h s e' val') :
-  val = val'.
-Proof.
-  eapply subst_exp_model' in HE1; [|eassumption].
-  rewrite HS in *.
-  apply HE1,HE2.
-Qed.
-
-Theorem trace_stmt_result' h P st st' st'' d q next ox
-        (HD : delta_models h d st st')
-        (HE : exec_stmt h st' q st'' ox)
-        (HN : match ox with
-              | None =>
-                  forall d' (HND : delta_models h d' st st''),
-                    match next d' with
-                    | Some tsl' => Exists P tsl'
-                    | None => True
-                    end
-              | Some x => True
-              end) :
-  match trace_stmt q next d with
-  | Some tsl => trace_states_modelo h P tsl st st'' ox
-  | None => True
-  end.
-Proof.
-  revert P st d next HD HN.
-  unfold trace_states_modelo in *.
-  induction HE; simpl in *; intros.
-  {
-    apply HN.
-    assumption.
-  }
-  {
-    apply HN.
+  Theorem subst_exp_model' h d s s' e val
+          (HST : delta_models h d s s')
+          (HE1 : eval_exp h s' e val) :
+    match subst_exp d e with
+    | Some e' => forall val' (HE2 : eval_exp h s e' val'), val = val'
+    | None => True
+    end.
+  Proof.
     rewrite delta_models_match in *.
-    intros v'.
-    rewrite delta_lookup_cons in *.
-    destruct iseq; subst; [|rewrite update_frame by assumption; apply HD].
-    rewrite update_updated.
-    eapply subst_exp_model'; [|eassumption].
-    apply delta_models_match.
-    assumption.
-  }
-  {
-    destruct subst_exp eqn:HS; [|tauto].
-    constructor.
+    revert d s HST.
+    induction HE1; simpl; intros.
+    1: {
+      apply HST.
+    }
+    7: {
+      apply IHHE1_2.
+      intro v'.
+      rewrite delta_lookup_cons in *.
+      destruct iseq; subst; [|rewrite update_frame by assumption; apply HST].
+      rewrite update_updated.
+      apply IHHE1_1.
+      assumption.
+    }
+    all:
+      repeat match goal with
+             | [IH : forall d _ _, match subst_exp d ?e with _ => _ end |- _] =>
+                 specialize (IH _ _ HST)
+             end.
+    8: destruct n1.
+    all:
+      repeat match goal with
+             | [|- context [match subst_exp _ _ with _ => _ end] ] =>
+                 destruct subst_exp
+             end; try solve [apply I].
+    all: intros; inversion HE2; subst.
+    all:
+      repeat match goal with
+             | [IH : forall _, (eval_exp _ _ ?e _) -> _ = _,
+                  E : eval_exp _ _ ?e _ |- _] =>
+                 specialize (IH _ E); inversion IH; subst
+             end; reflexivity.
+  Qed.
+
+  Theorem subst_exp_model h d s s' e val e' val'
+          (HST : delta_models h d s s')
+          (HS : subst_exp d e = Some e')
+          (HE1 : eval_exp h s' e val)
+          (HE2 : eval_exp h s e' val') :
+    val = val'.
+  Proof.
+    eapply subst_exp_model' in HE1; [|eassumption].
+    rewrite HS in *.
+    apply HE1,HE2.
+  Qed.
+
+  Theorem trace_stmt_result' h P st st' st'' d q next ox
+          (HD : delta_models h d st st')
+          (HE : exec_stmt h st' q st'' ox)
+          (HN : match ox with
+                | None =>
+                    forall d' (HND : delta_models h d' st st''),
+                      match next d' with
+                      | Some tsl' => Exists P tsl'
+                      | None => True
+                      end
+                | Some x => True
+                end) :
+    match trace_stmt q next d with
+    | Some tsl => trace_states_modelo h P tsl st st'' ox
+    | None => True
+    end.
+  Proof.
+    revert P st d next HD HN.
+    unfold trace_states_modelo in *.
+    induction HE; simpl in *; intros.
+    {
+      apply HN.
+      assumption.
+    }
+    {
+      apply HN.
+      rewrite delta_models_match in *.
+      intros v'.
+      rewrite delta_lookup_cons in *.
+      destruct iseq; subst; [|rewrite update_frame by assumption; apply HD].
+      rewrite update_updated.
+      eapply subst_exp_model'; [|eassumption].
+      apply delta_models_match.
+      assumption.
+    }
+    {
+      destruct subst_exp eqn:HS; [|tauto].
+      constructor.
+      simpl.
+      split; [assumption|].
+      intros.
+      eapply subst_exp_model in HS; try eassumption.
+      inversion HS; subst.
+      reflexivity.
+    }
+    {
+      constructor.
+      simpl.
+      tauto.
+    }
+    {
+      apply IHHE; assumption.
+    }
+    {
+      eapply IHHE1; [apply HD|].
+      intros.
+      apply IHHE2; assumption.
+    }
+    {
+      eapply IHHE in HD; [|apply HN].
+      destruct c; do 2 destruct trace_stmt; try apply I;
+        simpl; rewrite Exists_app; tauto.
+    }
+    {
+      apply I.
+    }
+  Qed.
+
+  Theorem trace_stmt_result h st st' st'' d q n ox tsl
+          (HD : delta_models h d st st')
+          (HE : exec_stmt h st' q st'' ox)
+          (HTS: trace_stmt q (trace_exit_res n) d = Some tsl) :
+    trace_states_model h tsl st st'' (exitof n ox).
+  Proof.
+    pose (P := fun ts => trace_state_models_exit h ts st st'' (Exit n)).
+    assert
+      (HX := trace_stmt_result' h P st st' st'' d q (trace_exit_res n) ox).
+    rewrite HTS in HX.
+    specialize (HX HD HE).
+    destruct ox; apply HX; [tauto|].
+    unfold P.
     simpl.
-    split; [assumption|].
     intros.
-    eapply subst_exp_model in HS; try eassumption.
-    inversion HS; subst.
-    reflexivity.
-  }
-  {
     constructor.
     simpl.
     tauto.
-  }
-  {
-    apply IHHE; assumption.
-  }
-  {
-    eapply IHHE1; [apply HD|].
+  Qed.
+
+  Theorem trace_result_consistent_exec h info tsl p a st st' time st'' x
+          (HC : trace_result_consistent h (info,tsl) p st)
+          (HInfo : info_models_loc h info a st st')
+          (HE : exec_prog h p a st' time st'' x) :
+    trace_result_models_exit h (info,tsl) st st'' x \/
+      exists time1 time2 st'x a',
+        time = (time1 + time2)%nat /\
+          exec_prog h p a st' time1 st'x (Exit a') /\
+          exec_prog h p a' st'x time2 st'' x /\
+          trace_states_model h tsl st st'x (Exit a').
+  Proof.
+    revert HInfo.
+    induction HE; simpl; [tauto| |]; intro.
+    {
+      assert (HCX := XS).
+      eapply HC in HCX; [|eassumption].
+      specialize (HCX LU).
+      simpl in *.
+      rewrite EX in *.
+      simpl in HCX.
+      destruct HCX as [HCX|HCX].
+      {
+        apply IHHE in HCX.
+        destruct HCX as [|[? [? [? [? [? [? [? ?] ] ] ] ] ] ] ]; [tauto|].
+        subst.
+        right.
+        eexists (S _).
+        do 3 econstructor.
+        repeat split; [|eassumption|eassumption].
+        econstructor; eassumption.
+      }
+      {
+        right.
+        exists (S 0).
+        simpl.
+        do 3 econstructor.
+        repeat split; [|eassumption|eassumption].
+        econstructor; [| | |constructor]; eassumption.
+      }
+    }
+    {
+      eapply HC in XS; [|eassumption].
+      apply XS in LU.
+      left.
+      assumption.
+    }
+  Qed.
+
+  Theorem trace_result_consistent_init h tsl p st :
+    trace_result_consistent h (treeN_nil,tsl) p st.
+  Proof.
+    simpl.
     intros.
-    apply IHHE2; assumption.
-  }
-  {
-    eapply IHHE in HD; [|apply HN].
-    destruct c; do 2 destruct trace_stmt; try apply I;
-      simpl; rewrite Exists_app; tauto.
-  }
-  {
-    apply I.
-  }
-Qed.
+    destruct a; compute in HInfo; tauto.
+  Qed.
 
-Theorem trace_stmt_result h st st' st'' d q n ox tsl
-        (HD : delta_models h d st st')
-        (HE : exec_stmt h st' q st'' ox)
-        (HTS: trace_stmt q (trace_exit_res n) d = Some tsl) :
-  trace_states_model h tsl st st'' (exitof n ox).
-Proof.
-  pose (P := fun ts => trace_state_models_exit h ts st st'' (Exit n)).
-  assert
-    (HX := trace_stmt_result' h P st st' st'' d q (trace_exit_res n) ox).
-  rewrite HTS in HX.
-  specialize (HX HD HE).
-  destruct ox; apply HX; [tauto|].
-  unfold P.
-  simpl.
-  intros.
-  constructor.
-  simpl.
-  tauto.
-Qed.
-
-Theorem trace_result_consistent_exec h info tsl p a st st' time st'' x
-        (HC : trace_result_consistent h (info,tsl) p st)
-        (HInfo : info_models_loc h info a st st')
-        (HE : exec_prog h p a st' time st'' x) :
-  trace_result_models_exit h (info,tsl) st st'' x \/
-    exists time1 time2 st'x a',
-      time = (time1 + time2)%nat /\
-        exec_prog h p a st' time1 st'x (Exit a') /\
-        exec_prog h p a' st'x time2 st'' x /\
-        trace_states_model h tsl st st'x (Exit a').
-Proof.
-  revert HInfo.
-  induction HE; simpl; [tauto| |]; intro.
-  {
-    assert (HCX := XS).
-    eapply HC in HCX; [|eassumption].
-    specialize (HCX LU).
-    simpl in *.
-    rewrite EX in *.
-    simpl in HCX.
-    destruct HCX as [HCX|HCX].
-    {
-      apply IHHE in HCX.
-      destruct HCX as [|[? [? [? [? [? [? [? ?] ] ] ] ] ] ] ]; [tauto|].
-      subst.
-      right.
-      eexists (S _).
-      do 3 econstructor.
-      repeat split; [|eassumption|eassumption].
-      econstructor; eassumption.
-    }
-    {
-      right.
-      exists (S 0).
-      simpl.
-      do 3 econstructor.
-      repeat split; [|eassumption|eassumption].
-      econstructor; [| | |constructor]; eassumption.
-    }
-  }
-  {
-    eapply HC in XS; [|eassumption].
-    apply XS in LU.
-    left.
-    assumption.
-  }
-Qed.
-
-Theorem trace_result_consistent_init h tsl p st :
-  trace_result_consistent h (treeN_nil,tsl) p st.
-Proof.
-  simpl.
-  intros.
-  destruct a; compute in HInfo; tauto.
-Qed.
-
-Theorem trace_step_modelled h p st tn tsl tnd d n
-        (HTN : treeN_lookup tn n = Some tnd)
-        (HLE : delta_le tnd d)
-        (HPrev : trace_result_consistent h (tn,(d,AELoc n)::tsl) p st) :
-  trace_result_consistent h (tn,tsl) p st.
-Proof.
-  unfold trace_result_consistent in *.
-  intros.
-  specialize (HPrev st' a st'' x sz q HInfo HE HP).
-  unfold trace_result_models_exit,trace_states_model in *.
-  rewrite Exists_cons in HPrev.
-  destruct HPrev as [?|[HPrev|?] ]; [tauto| |tauto].
-  unfold trace_state_models_exit in HPrev.
-  destruct exitof eqn:HEX; [|tauto].
-  destruct HPrev as [HPrev ?]; subst.
-  simpl.
-  unfold info_models_loc.
-  rewrite HTN.
-  left.
-  eapply delta_models_le; eassumption.
-Qed.
-
-Theorem trace_state_models_exit_promote_word h d n w st st' x
-        (HM : trace_state_models_exit h (d, AEExp (Word n w)) st st' x) :
-  trace_state_models_exit h (d, AELoc n) st st' x.
-Proof.
-  simpl in *.
-  destruct HM as [? HM].
-  split; [assumption|].
-  destruct x; [|tauto].
-  symmetry.
-  eapply HM.
-  constructor.
-Qed.
-
-Theorem trace_step_promote_word h p st tn tsl d n w
-        (HPrev : trace_result_consistent h (tn,(d,AEExp (Word n w))::tsl) p st) :
-  trace_result_consistent h (tn,(d,AELoc n)::tsl) p st.
-Proof.
-  unfold trace_result_consistent in *.
-  unfold trace_result_models_exit in *.
-  intros.
-  specialize (HPrev st' a st'' x sz q HInfo HE HP).
-  unfold trace_states_model in *.
-  rewrite Exists_cons in *.
-  destruct HPrev as [?|[HPrev|?] ]; [tauto| |tauto].
-  right.
-  left.
-  eapply trace_state_models_exit_promote_word.
-  eassumption.
-Qed.
-
-Theorem trace_step_stmt_consistent h p st tn d tsl tsl' n sz q
-        (od' := treeN_lookup tn n)
-        (dm := odelta_merge d od')
-        (HP : forall st' n, p st' n = p st n)
-        (HTX : p st n = Some (sz,q))
-        (HT : trace_stmt q (trace_exit_res (n + sz)) dm = Some tsl')
-        (HPrev : trace_result_consistent h (tn,(d,AELoc n)::tsl) p st) :
-  trace_inter_consistent h ((treeN_update tn n (Some dm),tsl),tsl') p st.
-Proof.
-  unfold dm,od' in *.
-  clear dm od'.
-  unfold trace_inter_consistent,trace_result_consistent in *.
-  intros st' a st'' x sz' q' HInfo HE HPX.
-  unfold trace_result_models_exit,trace_states_model in *.
-  rewrite Exists_app.
-  unfold info_models_loc in HInfo.
-  rewrite treeN_lookup_update in HInfo.
-  destruct (iseq n a) as [?|HX]; subst.
-  {
-    rewrite N.eqb_refl in HInfo.
-    rewrite HP in HPX.
-    rewrite HTX in HPX.
-    inversion HPX; subst.
-    right.
-    right.
-    eapply trace_stmt_result; eassumption.
-  }
-  {
-    apply N.eqb_neq in HX.
-    rewrite HX in HInfo.
-    specialize (HPrev st' a st'' x sz' q' HInfo HE HPX).
+  Theorem trace_step_modelled h p st tn tsl tnd d n
+          (HTN : treeN_lookup tn n = Some tnd)
+          (HLE : delta_le tnd d)
+          (HPrev : trace_result_consistent h (tn,(d,AELoc n)::tsl) p st) :
+    trace_result_consistent h (tn,tsl) p st.
+  Proof.
+    unfold trace_result_consistent in *.
+    intros.
+    specialize (HPrev st' a st'' x sz q HInfo HE HP).
+    unfold trace_result_models_exit,trace_states_model in *.
     rewrite Exists_cons in HPrev.
-    destruct HPrev as [HPrev|[HPrev|?] ]; [| |tauto].
+    destruct HPrev as [?|[HPrev|?] ]; [tauto| |tauto].
+    unfold trace_state_models_exit in HPrev.
+    destruct exitof eqn:HEX; [|tauto].
+    destruct HPrev as [HPrev ?]; subst.
+    simpl.
+    unfold info_models_loc.
+    rewrite HTN.
+    left.
+    eapply delta_models_le; eassumption.
+  Qed.
+
+  Theorem trace_state_models_exit_promote_word h d n w st st' x
+          (HM : trace_state_models_exit h (d, AEExp (Word n w)) st st' x) :
+    trace_state_models_exit h (d, AELoc n) st st' x.
+  Proof.
+    simpl in *.
+    destruct HM as [? HM].
+    split; [assumption|].
+    destruct x; [|tauto].
+    symmetry.
+    eapply HM.
+    constructor.
+  Qed.
+
+  Theorem trace_step_promote_word h p st tn tsl d n w
+          (HPrev : trace_result_consistent h (tn,(d,AEExp (Word n w))::tsl) p st) :
+    trace_result_consistent h (tn,(d,AELoc n)::tsl) p st.
+  Proof.
+    unfold trace_result_consistent in *.
+    unfold trace_result_models_exit in *.
+    intros.
+    specialize (HPrev st' a st'' x sz q HInfo HE HP).
+    unfold trace_states_model in *.
+    rewrite Exists_cons in *.
+    destruct HPrev as [?|[HPrev|?] ]; [tauto| |tauto].
+    right.
+    left.
+    eapply trace_state_models_exit_promote_word.
+    eassumption.
+  Qed.
+
+  Theorem trace_step_stmt_consistent h p st tn d tsl tsl' n sz q
+          (od' := treeN_lookup tn n)
+          (dm := odelta_merge d od')
+          (HP : forall st' n, p st' n = p st n)
+          (HTX : p st n = Some (sz,q))
+          (HT : trace_stmt q (trace_exit_res (n + sz)) dm = Some tsl')
+          (HPrev : trace_result_consistent h (tn,(d,AELoc n)::tsl) p st) :
+    trace_inter_consistent h ((treeN_update tn n (Some dm),tsl),tsl') p st.
+  Proof.
+    unfold dm,od' in *.
+    clear dm od'.
+    unfold trace_inter_consistent,trace_result_consistent in *.
+    intros st' a st'' x sz' q' HInfo HE HPX.
+    unfold trace_result_models_exit,trace_states_model in *.
+    rewrite Exists_app.
+    unfold info_models_loc in HInfo.
+    rewrite treeN_lookup_update in HInfo.
+    destruct (iseq n a) as [?|HX]; subst.
     {
-      left.
-      destruct exitof as [a'|]; [|tauto].
-      simpl in *.
-      unfold info_models_loc in *.
-      rewrite treeN_lookup_update.
-      destruct (n =? a') eqn:HXX; [|assumption].
-      apply Neqb_ok in HXX.
-      subst.
-      destruct (treeN_lookup tn a'); [|tauto].
-      eapply delta_models_le; [|eassumption].
-      apply delta_merge_le_r.
+      rewrite N.eqb_refl in HInfo.
+      rewrite HP in HPX.
+      rewrite HTX in HPX.
+      inversion HPX; subst.
+      right.
+      right.
+      eapply trace_stmt_result; eassumption.
     }
     {
-      left.
-      simpl in *.
-      destruct HPrev as [HM ?].
-      destruct exitof; [subst|tauto].
-      simpl in *.
-      unfold info_models_loc.
-      rewrite treeN_update_updated.
-      destruct treeN_lookup; [|assumption].
-      eapply delta_models_le; [|eassumption].
-      apply delta_merge_le_l.
+      apply N.eqb_neq in HX.
+      rewrite HX in HInfo.
+      specialize (HPrev st' a st'' x sz' q' HInfo HE HPX).
+      rewrite Exists_cons in HPrev.
+      destruct HPrev as [HPrev|[HPrev|?] ]; [| |tauto].
+      {
+        left.
+        destruct exitof as [a'|]; [|tauto].
+        simpl in *.
+        unfold info_models_loc in *.
+        rewrite treeN_lookup_update.
+        destruct (n =? a') eqn:HXX; [|assumption].
+        apply Neqb_ok in HXX.
+        subst.
+        destruct (treeN_lookup tn a'); [|tauto].
+        eapply delta_models_le; [|eassumption].
+        apply delta_merge_le_r.
+      }
+      {
+        left.
+        simpl in *.
+        destruct HPrev as [HM ?].
+        destruct exitof; [subst|tauto].
+        simpl in *.
+        unfold info_models_loc.
+        rewrite treeN_update_updated.
+        destruct treeN_lookup; [|assumption].
+        eapply delta_models_le; [|eassumption].
+        apply delta_merge_le_l.
+      }
     }
-  }
-Qed.
+  Qed.
 
-Theorem trace_step_models_consistent h p st tn tsl ts
-        (HP : forall st' n, p st' n = p st n)
-        (HPrev : trace_result_consistent h (tn,ts::tsl) p st) :
-  trace_inter_consistent h (step_trace (p st) (tn,tsl) ts) p st.
-Proof.
-  assert (HSkip : trace_inter_consistent h ((tn,ts::tsl),nil) p st)
-    by (simpl; rewrite app_nil_r; assumption).
-  simpl.
-  destruct ts as [d ae].
-  destruct ae; [|assumption|assumption].
-  destruct p as [ [? ?]|] eqn:HPX1; [|assumption].
-  destruct odelta_leb eqn:HL.
-  {
-    unfold trace_inter_consistent.
-    rewrite app_nil_r.
-    unfold odelta_leb in HL.
-    destruct treeN_lookup eqn:?; [|discriminate].
-    apply delta_le_leb in HL.
-    eapply trace_step_modelled; eassumption.
-  }
-  {
-    destruct trace_stmt eqn:HTR; [|assumption].
-    eapply trace_step_stmt_consistent; eassumption.
-  }
-Qed.
+  Theorem trace_step_models_consistent h p st tn tsl ts
+          (HP : forall st' n, p st' n = p st n)
+          (HPrev : trace_result_consistent h (tn,ts::tsl) p st) :
+    trace_inter_consistent h (step_trace (p st) (tn,tsl) ts) p st.
+  Proof.
+    assert (HSkip : trace_inter_consistent h ((tn,ts::tsl),nil) p st)
+      by (simpl; rewrite app_nil_r; assumption).
+    simpl.
+    destruct ts as [d ae].
+    destruct ae; [|assumption|assumption].
+    destruct p as [ [? ?]|] eqn:HPX1; [|assumption].
+    destruct odelta_leb eqn:HL.
+    {
+      unfold trace_inter_consistent.
+      rewrite app_nil_r.
+      unfold odelta_leb in HL.
+      destruct treeN_lookup eqn:?; [|discriminate].
+      apply delta_le_leb in HL.
+      eapply trace_step_modelled; eassumption.
+    }
+    {
+      destruct trace_stmt eqn:HTR; [|assumption].
+      eapply trace_step_stmt_consistent; eassumption.
+    }
+  Qed.
 
-Theorem eval_expeq_altdef_bad h st
-        (expeq : forall e1 e2, Prop)
-        (* (expeq_symm : forall e1 e2, expeq e1 e2 -> expeq e2 e1) *)
-        (expeq_refl : forall e, expeq e e)
-        (* (expeq_trans : *)
-        (*   forall e1 e2 e3, expeq e1 e2 -> expeq e2 e3 -> expeq e1 e3) *)
-        (eval_expeq :
-          forall e1 e2 v1 v2
-                 (HEq : expeq e1 e2)
-                 (HE1 : eval_exp h st e1 v1)
-                 (HE2 : eval_exp h st e2 v2),
-            v1 = v2) :
-  False.
-Proof.
-  specialize (eval_expeq (Unknown 1) _ (VaN 0 1) (VaN 1 1) (expeq_refl _)).
-  assert (HX : VaN 0 1 <> VaN 1 1) by (intro BAD; inversion BAD).
-  apply HX,eval_expeq; constructor; reflexivity.
-Qed.
+  Theorem eval_expeq_altdef_bad h st
+          (expeq : forall e1 e2, Prop)
+          (* (expeq_symm : forall e1 e2, expeq e1 e2 -> expeq e2 e1) *)
+          (expeq_refl : forall e, expeq e e)
+          (* (expeq_trans : *)
+          (*   forall e1 e2 e3, expeq e1 e2 -> expeq e2 e3 -> expeq e1 e3) *)
+          (eval_expeq :
+            forall e1 e2 v1 v2
+                   (HEq : expeq e1 e2)
+                   (HE1 : eval_exp h st e1 v1)
+                   (HE2 : eval_exp h st e2 v2),
+              v1 = v2) :
+    False.
+  Proof.
+    specialize (eval_expeq (Unknown 1) _ (VaN 0 1) (VaN 1 1) (expeq_refl _)).
+    assert (HX : VaN 0 1 <> VaN 1 1) by (intro BAD; inversion BAD).
+    apply HX,eval_expeq; constructor; reflexivity.
+  Qed.
+End PICINAE_CALLING.
+
+Module PICINAE_CALLING_DEFS_EQ (IL : PICINAE_IL) <: PICINAE_CALLING_DEFS IL.
+  Import IL.
+
+  Program Instance endian_EqDec: EqDec endianness.
+  Next Obligation. Proof. decide equality. Defined.
+
+  Program Instance binop_EqDec: EqDec binop_typ.
+  Next Obligation. Proof. decide equality. Defined.
+
+  Program Instance unop_EqDec: EqDec unop_typ.
+  Next Obligation. Proof. decide equality. Defined.
+
+  Program Instance cast_EqDec: EqDec cast_typ.
+  Next Obligation. Proof. decide equality. Defined.
+
+  Program Instance bool_EqDec : EqDec bool.
+  Next Obligation. Proof. decide equality. Defined.
+
+  Program Instance option_EqDec A `(EA : EqDec A) : EqDec (option A).
+  Next Obligation. Proof. decide equality. apply iseq. Defined.
+
+  Program Instance tuple_EqDec A B `(EA : EqDec A) `(EA : EqDec B): EqDec (A * B).
+  Next Obligation. Proof. decide equality; apply iseq. Defined.
+
+  Program Instance list_EqDec A `(EA : EqDec A) : EqDec (list A).
+  Next Obligation. Proof. decide equality. apply iseq. Defined.
+
+  Program Instance exp_EqDec: EqDec exp.
+  Next Obligation. Proof. decide equality; apply iseq. Defined.
+
+  Definition expeq (e1 e2 : exp) := e1 = e2.
+  Definition expeqb e1 e2 := if e1 == e2 then true else false.
+  Theorem expeqb_expeq e1 e2 : expeqb e1 e2 = true <-> expeq e1 e2.
+  Proof.
+    unfold expeqb,expeq.
+    destruct iseq; intuition.
+  Qed.
+  Theorem expeq_symm e1 e2 (HEq : expeq e1 e2) : expeq e2 e1.
+  Proof.
+    unfold expeq in *.
+    subst.
+    reflexivity.
+  Qed.
+  Theorem expeq_trans e1 e2 e3 (HEq1 : expeq e1 e2) (HEq2 : expeq e2 e3) :
+    expeq e1 e3.
+  Proof.
+    unfold expeq in *.
+    subst.
+    reflexivity.
+  Qed.
+  Definition expeq_refl (e : exp) := eq_refl e.
+  Theorem eval_expeq h st e1 e2 v (HEq : expeq e1 e2) (HE : eval_exp h st e1 v) :
+    eval_exp h st e2 v.
+  Proof.
+    unfold expeq in *.
+    subst.
+    assumption.
+  Qed.
+End PICINAE_CALLING_DEFS_EQ.
